%\Huge
%
%$u_i = \bar{u}_i + u_i'$
%
%\
%
%$\phi = \bar{\phi} + \phi'$
%
%\
%
%$ SST \ \ \ k-\omega \ \ \ \ k-\epsilon \ \ \ \ LES \ \ \ \ TLES \ \ \ DNS$
%
%\
%
%$$
%\dfrac{\partial \rho}{\partial t} + \dfrac{\partial}{\partial x_i}(\rho u_i)=0
%$$
%
%\
%
%\begin{equation}
%\dfrac{1}{\rho_q}\bigg[ \dfrac{\partial}{\partial t}(\alpha_q \rho_q)+ \nabla\cdot (\alpha_q\rho_q \hat{u}_q)\ = S_{\alpha_q} \sum^n_{p=1} (\dot{m}_{pq} - \dot{m}_{qp})\bigg]
%\end{equation}
%
%$$
%\dfrac{\partial}{\partial t}(\rho \hat{u}) + \nabla \cdot (\rho \hat{u} \hat{u}) = - \nabla p + \nabla \cdot \big[\mu (\nabla \hat{u} + \nabla \hat{u}^T)\big]+ \rho g+ F
%$$

\begin{figure}
\centering
\includegraphics[width=0.8\textwidth]{figuras/fluxograma}
\end{figure}